tweak state_interp, run_yield_1 adequacy wip

theories/RAs.v
@@ -7,46 +7,48 @@ From stdpp Require Import fin_maps.
 
   Class gen_VMPreG (A V W R P F: Type) (Σ:gFunctors)
         `{Countable A, Countable V, Countable W, Countable R, Countable P} := {
-                      gen_token_preG_inG :> inG Σ (frac_authR (agreeR (leibnizO V)));
-                      gen_mem_preG_inG :> gen_heapGpreS A W Σ;
-                      gen_reg_preG_inG :> gen_heapGpreS (R * V) W Σ;
-                      gen_tx_preG_inG :> inG Σ (authR (gmapUR V (agreeR (leibnizO P))));
-                      gen_rx_preG_inG :> inG Σ (prodR (authR (gmapUR V (agreeR (leibnizO P))))
-                                                      (optionR (gmap_viewR V (optionO (prodO (leibnizO W) (leibnizO V))))));
-                      gen_owned_preG_inG :> inG Σ (authR (gmapUR V
-                                                    (prodR dfracR (agreeR (gset_disjUR (leibnizO P))))));
-                      gen_access_preG_inG :> inG Σ (authR (gmapUR V
-                                                    (prodR dfracR (agreeR (gset_disjUR (leibnizO P))))));
-                      gen_excl_preG_inG :> inG Σ (authR (gmapUR V
-                                                    (prodR dfracR (agreeR (gset_disjUR (leibnizO P))))));
-                      gen_trans_preG_inG :> gen_heapGpreS W (V * W*  V * (list P)*F) Σ;
-                      gen_hpool_preG_inG :> inG Σ (frac_authR (gset_disjR (leibnizO W)));
-                      gen_retri_preG_inG :> gen_heapGpreS W bool Σ
-                   }.
+    gen_token_preG_inG :> inG Σ (frac_authR (agreeR (leibnizO V)));
+    gen_mem_preG_inG :> gen_heapGpreS A W Σ;
+    gen_reg_preG_inG :> gen_heapGpreS (R * V) W Σ;
+    gen_tx_preG_inG :> inG Σ (authR (gmapUR V (agreeR (leibnizO P))));
+    gen_rx_agree_preG_inG :> inG Σ (authR (gmapUR V (agreeR (leibnizO P))));
+    gen_rx_option_preG_inG :> gen_heapGpreS V (option (W * V)) Σ;
+    gen_owned_preG_inG :> inG Σ (authR (gmapUR V
+                                               (prodR dfracR (agreeR (gset_disjUR (leibnizO P))))));
+    gen_access_preG_inG :> inG Σ (authR (gmapUR V
+                                                (prodR dfracR (agreeR (gset_disjUR (leibnizO P))))));
+    gen_excl_preG_inG :> inG Σ (authR (gmapUR V
+                                              (prodR dfracR (agreeR (gset_disjUR (leibnizO P))))));
+    gen_trans_preG_inG :> gen_heapGpreS W (V * W*  V * (list P)*F) Σ;
+    gen_hpool_preG_inG :> inG Σ (frac_authR (gset_disjR (leibnizO W)));
+    gen_retri_preG_inG :> gen_heapGpreS W bool Σ
+    }.
 
 
   Class gen_VMG Σ := GenVMG{
-                      gen_VM_inG :> gen_VMPreG Addr VMID Word reg_name PID transaction_type Σ;
-                      gen_invG :> invGS Σ;
-                      gen_na_invG :> na_invG Σ;
-                      gen_nainv_name : na_inv_pool_name;
-                      gen_token_name : gname;
-                      gen_mem_name : gname;
-                      gen_reg_name : gname;
-                      gen_tx_name : gname;
-                      gen_rx_name : gname;
-                      gen_owned_name : gname;
-                      gen_access_name : gname;
-                      gen_excl_name : gname;
-                      gen_trans_name : gname;
-                      gen_hpool_name : gname;
-                      gen_retri_name : gname
-                    }.
+                         gen_VM_inG :> gen_VMPreG Addr VMID Word reg_name PID transaction_type Σ;
+                         gen_invG :> invGS Σ;
+                         gen_na_invG :> na_invG Σ;
+                         gen_nainv_name : na_inv_pool_name;
+                         gen_token_name : gname;
+                         gen_mem_name : gname;
+                         gen_reg_name : gname;
+                         gen_tx_name : gname;
+                         gen_rx_agree_name : gname;
+                         gen_rx_option_name : gname;
+                         gen_owned_name : gname;
+                         gen_access_name : gname;
+                         gen_excl_name : gname;
+                         gen_trans_name : gname;
+                         gen_hpool_name : gname;
+                         gen_retri_name : gname
+                       }.
 Global Arguments gen_nainv_name {Σ} _.
 Global Arguments gen_token_name {Σ} _.
 Global Arguments gen_mem_name {Σ} _.
 Global Arguments gen_reg_name {Σ} _.
-Global Arguments gen_rx_name {Σ} _.
+Global Arguments gen_rx_agree_name {Σ} _.
+Global Arguments gen_rx_option_name {Σ} _.
 Global Arguments gen_tx_name {Σ} _.
 Global Arguments gen_owned_name {Σ} _.
 Global Arguments gen_access_name {Σ} _.
@@ -55,12 +57,11 @@ Global Arguments gen_trans_name {Σ} _.
 Global Arguments gen_hpool_name {Σ} _.
 Global Arguments gen_retri_name {Σ} _.
 
-Definition ra_tx :=
+Definition ra_rx_tx_agree :=
   (authR (gmapUR VMID (agreeR (leibnizO PID)))).
 
 Definition ra_rx :=
-  (prodR ra_tx
-         (optionR (gmap_viewR VMID (optionO (prodO (leibnizO Word) (leibnizO VMID)))))).
+  (gmap VMID (option (Word*VMID))).
 
 Definition ra_page_table:=
   (authR (gmapUR VMID (prodR dfracR (agreeR (gset_disjUR (leibnizO PID)))))).
@@ -68,19 +69,20 @@ Definition ra_page_table:=
 
 Definition gen_VMΣ : gFunctors :=
   #[
-      invΣ;
-      na_invΣ;
-      GFunctor (frac_authR (agreeR (leibnizO VMID)));
-      gen_heapΣ Addr Word;
-      gen_heapΣ (reg_name * VMID) Word;
-      GFunctor ra_tx;
-      GFunctor ra_rx;
-      GFunctor ra_page_table;
-      GFunctor ra_page_table;
-      GFunctor ra_page_table;
-      gen_heapΣ Word (VMID * Word *  VMID * (list PID) * transaction_type);
-      GFunctor (frac_authR (gset_disjR (leibnizO Word)));
-      gen_heapΣ Word bool
+    invΣ;
+    na_invΣ;
+    GFunctor (frac_authR (agreeR (leibnizO VMID)));
+    gen_heapΣ Addr Word;
+    gen_heapΣ (reg_name * VMID) Word;
+    GFunctor ra_rx_tx_agree;
+    GFunctor ra_rx_tx_agree;
+    gen_heapΣ VMID (option (Word*VMID));
+    GFunctor ra_page_table;
+    GFunctor ra_page_table;
+    GFunctor ra_page_table;
+    gen_heapΣ Word (VMID * Word *  VMID * (list PID) * transaction_type);
+    GFunctor (frac_authR (gset_disjR (leibnizO Word)));
+    gen_heapΣ Word bool
    ].
 
 Global Instance subG_gen_VMPreG {Σ}:
@@ -116,21 +118,19 @@ Section definitions.
   Definition get_reg_gmap σ: gmap (reg_name * VMID) Word :=
      (list_to_map (flat_map (λ v, (map (λ p, ((p.1,v),p.2)) (map_to_list (get_vm_reg_file σ v)))) (list_of_vmids))).
 
-  Definition get_txrx_auth_agree σ (f: mail_box -> PID) : ra_tx:=
-    (● (list_to_map (map (λ v, (v,to_agree (f (get_vm_mail_box σ v)))) (list_of_vmids) )
-    )).
+  Definition get_txrx_auth_agree σ (f: mail_box -> PID) :(gmap VMID (agreeR (leibnizO PID))) :=
+    (list_to_map (map (λ v, (v,to_agree (f (get_vm_mail_box σ v)))) (list_of_vmids))).
 
   Definition get_tx_agree σ := get_txrx_auth_agree σ (λ p, p.1).
 
   Definition get_rx_agree σ := get_txrx_auth_agree σ (λ p, p.2.1).
 
-  Definition get_rx_gmap σ :=
-    (Some (gmap_view_auth 1
+  Definition get_rx_gmap σ : gmap VMID _ :=
             ((list_to_map (map (λ v, let mb := (get_vm_mail_box σ v) in
                                     match mb.2.2 with
                                       | Some (l, j) => (v, (Some ( l, j)))
                                       | None => (v,None)
-                                    end) (list_of_vmids))): (gmap VMID (optionO (prodO (leibnizO Word) (leibnizO VMID))) )))).
+                                    end) (list_of_vmids)))).
 
   Definition get_pagetable_gmap{Perm: Type} σ (proj: page_table -> gmap PID Perm)
              (checkb: Perm -> bool)
@@ -164,8 +164,9 @@ Section definitions.
       own (gen_token_name vmG) (get_token (get_current_vm σ)) ∗
       ghost_map_auth (gen_mem_name vmG) 1 (get_mem σ) ∗
       ghost_map_auth (gen_reg_name vmG) 1 (get_reg_gmap σ) ∗
-      own (gen_tx_name vmG) (get_tx_agree σ) ∗
-      own (gen_rx_name vmG) ((get_rx_agree σ), (get_rx_gmap σ) )∗
+      own (gen_tx_name vmG) (● (get_tx_agree σ)) ∗
+      own (gen_rx_agree_name vmG) (● (get_rx_agree σ)) ∗
+      ghost_map_auth (gen_rx_option_name vmG) 1 (get_rx_gmap σ) ∗
       own (gen_owned_name vmG)  (●(get_owned_gmap σ)) ∗
       own (gen_access_name vmG) (● (get_access_gmap σ)) ∗
       own (gen_excl_name vmG) (●(get_excl_gmap σ)) ∗
@@ -199,24 +200,19 @@ Section definitions.
   Definition tx_mapsto := tx_mapsto_aux.(unseal).
   Definition tx_mapsto_eq : @tx_mapsto = @tx_mapsto_def := tx_mapsto_aux.(seal_eq).
 
-  Definition rx_mapsto_def1 (i:VMID) (p:PID) (nr : option (Word *  VMID)) : iProp Σ :=
-    match nr with
-      | Some (n, r) =>
-        own (gen_rx_name vmG) ((◯ {[i := (to_agree p)]}),
-                               (Some (gmap_view_frag i (DfracOwn 1) (Some ((n:(leibnizO Word)), (r: leibnizO VMID))))))
-      | None =>
-        own (gen_rx_name vmG) ((◯ {[i := (to_agree p)]}),
-                               (Some (gmap_view_frag i (DfracOwn 1) None)))
-    end.
-  Definition rx_mapsto_aux1 : seal (@rx_mapsto_def1). Proof. by eexists. Qed.
-  Definition rx_mapsto1 := rx_mapsto_aux1.(unseal).
-  Definition rx_mapsto_eq1 : @rx_mapsto1 = @rx_mapsto_def1 := rx_mapsto_aux1.(seal_eq).
+  Definition rx_option_mapsto_def (i:VMID) (nr : option (Word *  VMID)) : iProp Σ :=
+    ghost_map_elem  (gen_rx_option_name vmG) i (DfracOwn 1) nr.
+  Definition rx_option_mapsto_aux : seal (@rx_option_mapsto_def). Proof. by eexists. Qed.
+  Definition rx_option_mapsto := rx_option_mapsto_aux.(unseal).
+  Definition rx_option_mapsto_eq : @rx_option_mapsto = @rx_option_mapsto_def :=
+    rx_option_mapsto_aux.(seal_eq).
 
-  Definition rx_mapsto_def2 (i:VMID) (p:PID) : iProp Σ :=
-    own (gen_rx_name vmG) ((◯ {[i := (to_agree p)]}),None).
-  Definition rx_mapsto_aux2 : seal (@rx_mapsto_def2). Proof. by eexists. Qed.
-  Definition rx_mapsto2 := rx_mapsto_aux2.(unseal).
-  Definition rx_mapsto_eq2 : @rx_mapsto2 = @rx_mapsto_def2 := rx_mapsto_aux2.(seal_eq).
+  Definition rx_agree_mapsto_def (i:VMID) (p:PID) : iProp Σ :=
+    own (gen_rx_agree_name vmG) (◯ {[i := (to_agree p)]}).
+  Definition rx_agree_mapsto_aux : seal (@rx_agree_mapsto_def). Proof. by eexists. Qed.
+  Definition rx_agree_mapsto := rx_agree_mapsto_aux.(unseal).
+  Definition rx_agree_mapsto_eq : @rx_agree_mapsto = @rx_agree_mapsto_def :=
+    rx_agree_mapsto_aux.(seal_eq).
 
   Definition owned_mapsto_def (i:VMID) dq (s: gset_disj PID) : iProp Σ :=
     own (gen_owned_name vmG) (◯ {[i := (dq, to_agree s)]}).
@@ -279,11 +275,11 @@ Notation "a ->a w" := (mem_mapsto a (DfracOwn 1) w) (at level 20) : bi_scope.
 (* predicates for TX and RX *)
 Notation "TX@ i := p" := (tx_mapsto i p)
                               (at level 20, format "TX@ i := p"): bi_scope.
-Notation "RX@ i :=( p ! n , r )" := (rx_mapsto1 i p (Some (n, r)))
+Notation "RX@ i :=( p ! n , r )" := ((rx_agree_mapsto i p) ∗ (rx_option_mapsto i (Some (n,r))))%I
                                         (at level 20, format "RX@ i :=( p ! n , r )"):bi_scope.
-Notation "RX@ i :=( p !)" := (rx_mapsto1 i p None)
+Notation "RX@ i :=( p !)" := ((rx_agree_mapsto i p) ∗ (rx_option_mapsto i None))%I
                                         (at level 20, format "RX@ i :=( p !)"):bi_scope.
-Notation "RX@ i := p " := (rx_mapsto2 i p)
+Notation "RX@ i := p " := (rx_agree_mapsto i p)
                                         (at level 20, format "RX@ i := p"):bi_scope.
 
 (* predicates for pagetables *)
@@ -319,16 +315,28 @@ Section hyp_lang_rules.
   Implicit Types w: Word.
 
   Lemma nainv_alloc γ E P :  ▷ P ={E}=∗ na_inv (gen_nainv_name vmG) γ P.
-    Proof.
-      iIntros "P".
-      iMod ((na_inv_alloc (gen_nainv_name vmG) E γ P) with "P") as "H".
-      done.
-    Qed.
+  Proof.
+    iIntros "P".
+    iMod ((na_inv_alloc (gen_nainv_name vmG) E γ P) with "P") as "H".
+    done.
+  Qed.
+
+  Lemma token_alloc i : ⊢ |==> ∃ γ, own γ (get_token i) ∗ own γ (frac_auth_frag 1%Qp (to_agree (i: leibnizO VMID))).
+  Proof.
+    iIntros.
+    rewrite /get_token.
+    iDestruct (own_alloc ((●F (to_agree (i: leibnizO VMID))) ⋅ (◯F (to_agree (i: leibnizO VMID))))) as ">Halloc".
+    { apply frac_auth_valid. done. }
+    iModIntro.
+    iDestruct "Halloc" as (γ) "Halloc".
+    iExists γ.
+    rewrite own_op //.
+  Qed.
 
   Lemma token_frag_valid i1 i2 q1 q2 :
    << i1 >>{ q1 } -∗
-      << i2 >>{ q2 } -∗
-      ⌜ i1 = i2 ⌝ ∧ ⌜ ((q1 + q2) ≤ 1)%Qp ⌝.
+   << i2 >>{ q2 } -∗
+   ⌜ i1 = i2 ⌝ ∧ ⌜ ((q1 + q2) ≤ 1)%Qp ⌝.
   Proof.
     rewrite token_agree_eq /token_agree_def.
     iIntros "H1 H2".
@@ -339,13 +347,12 @@ Section hyp_lang_rules.
     destruct Hvalid.
     apply to_agree_op_inv_L in H0.
     done.
-   Qed.
-
+  Qed.
 
   Lemma token_frag_split i q1 q2 :
    (q1 + q2 = 1)%Qp ->
    << i >>{ 1%Qp } -∗
-      << i >>{ q1 } ∗ << i >>{ q2}.
+   << i >>{ q1 } ∗ << i >>{ q2}.
   Proof.
     intro.
     rewrite token_agree_eq /token_agree_def.
@@ -354,11 +361,11 @@ Section hyp_lang_rules.
     rewrite -frac_auth_frag_op.
     rewrite H.
     by rewrite agree_idemp.
-   Qed.
+  Qed.
 
-   Lemma token_frag_merge i q1 q2 :
+  Lemma token_frag_merge i q1 q2 :
    (q2 + q1 = 1)%Qp ->
-      << i >>{ q1 } -∗ << i >>{ q2} -∗
+   << i >>{ q1 } -∗ << i >>{ q2} -∗
    << i >>{ 1%Qp }.
   Proof.
     intro.
@@ -369,13 +376,12 @@ Section hyp_lang_rules.
     rewrite -frac_auth_frag_op.
     rewrite H.
     by rewrite agree_idemp.
-   Qed.
+  Qed.
 
-
-   Lemma token_auth_valid i1 i2 q :
+  Lemma token_auth_valid i1 i2 q :
    << i1 >>{ q } -∗
-      (own (gen_token_name vmG) (get_token i2)%I) -∗
-      ⌜ i1 = i2 ⌝.
+   (own (gen_token_name vmG) (get_token i2)%I) -∗
+   ⌜ i1 = i2 ⌝.
   Proof.
     rewrite token_agree_eq /token_agree_def.
     iIntros "H1 H2".
@@ -385,13 +391,12 @@ Section hyp_lang_rules.
     apply to_agree_included in Hvalid.
     destruct Hvalid.
     done.
-   Qed.
+  Qed.
 
-
-    Lemma token_update i1 i2 i3 :
+  Lemma token_update i1 i2 i3 :
    << i1 >>{ 1%Qp } -∗
-      (own (gen_token_name vmG) (get_token i2))  ==∗
-      << i3 >>{ 1%Qp } ∗ (own (gen_token_name vmG) (get_token i3)).
+   (own (gen_token_name vmG) (get_token i2))  ==∗
+   << i3 >>{ 1%Qp } ∗ (own (gen_token_name vmG) (get_token i3)).
   Proof.
     rewrite token_agree_eq /token_agree_def /get_token.
     rewrite -own_op.
@@ -400,7 +405,7 @@ Section hyp_lang_rules.
    done.
   Qed.
 
-   Lemma gen_token_valid_neq{σ q} i j:
+  Lemma gen_token_valid_neq{σ q} i j:
    i ≠ j ->
    << i >>{ q } -∗
    own (gen_token_name vmG) (get_token (get_current_vm σ)) -∗
@@ -440,32 +445,39 @@ Section hyp_lang_rules.
     - iLeft. done.
   Qed.
 
-Lemma gen_reg_valid1:
-  ∀ (σ : state) r i w,
-    (get_current_vm σ) = i ->
-    ghost_map_auth (gen_reg_name vmG) 1 (get_reg_gmap σ) -∗
-    r @@ i ->r w -∗
-          ⌜ (get_reg σ r) = Some w ⌝.
-Proof.
-  iIntros (?????) "Hσ Hr".
-  rewrite reg_mapsto_eq /reg_mapsto_def.
-  iDestruct (ghost_map_lookup with "Hσ Hr") as "%".
-  iPureIntro.
-  rewrite /get_reg /get_reg_global.
-  unfold get_reg_gmap in H0.
-  apply elem_of_list_to_map_2 in H0.
-  apply elem_of_list_In in H0.
-  apply in_flat_map in H0.
-  inversion H0; clear H0.
-  destruct H1.
-  apply in_map_iff in H1.
-  inversion H1;clear H1.
-  inversion H2;clear H2.
-  inversion H1.
-  apply elem_of_list_In in H3.
-  apply elem_of_map_to_list' in H3.
-  by simplify_eq /=.
-Qed.
+  Lemma gen_reg_alloc (regs: gmap (reg_name * VMID) Word) :
+   ⊢ |==> ∃ γ, ghost_map_auth γ 1%Qp regs ∗
+               [∗ map] p↦w∈ regs, ghost_map_elem γ p (DfracOwn 1%Qp) w.
+  Proof.
+    iApply ghost_map_alloc.
+  Qed.
+
+  Lemma gen_reg_valid1:
+   ∀ (σ : state) r i w,
+     (get_current_vm σ) = i ->
+     ghost_map_auth (gen_reg_name vmG) 1 (get_reg_gmap σ) -∗
+     r @@ i ->r w -∗
+     ⌜ (get_reg σ r) = Some w ⌝.
+  Proof.
+    iIntros (?????) "Hσ Hr".
+    rewrite reg_mapsto_eq /reg_mapsto_def.
+    iDestruct (ghost_map_lookup with "Hσ Hr") as "%".
+    iPureIntro.
+    rewrite /get_reg /get_reg_global.
+    unfold get_reg_gmap in H0.
+    apply elem_of_list_to_map_2 in H0.
+    apply elem_of_list_In in H0.
+    apply in_flat_map in H0.
+    inversion H0; clear H0.
+    destruct H1.
+    apply in_map_iff in H1.
+    inversion H1;clear H1.
+    inversion H2;clear H2.
+    inversion H1.
+    apply elem_of_list_In in H3.
+    apply elem_of_map_to_list' in H3.
+    by simplify_eq /=.
+  Qed.
 
 
 Lemma gen_reg_valid_global1:
@@ -530,30 +542,29 @@ Proof.
   by simplify_eq /=.
 Qed.
 
-Lemma gen_reg_valid2:
-  ∀ (σ : state) i r1 w1 r2 w2 ,
-    (get_current_vm σ) = i ->
-    r1 ≠ r2->
-    ghost_map_auth (gen_reg_name vmG) 1 (get_reg_gmap σ) -∗
-                r1 @@ i ->r w1 -∗
-                             r2 @@ i ->r w2 -∗
-           ⌜ (get_reg σ r1) = Some w1 ⌝ ∗ ⌜ (get_reg σ r2) =Some w2 ⌝.
-Proof.
-  iIntros (?????? Hneq Hi) "Hreg Hr1 Hr2".
-  iDestruct ((gen_reg_valid_Sep σ i (<[(r1,i):=w1]>{[(r2,i):=w2]}))
-               with "Hreg [Hr1 Hr2]") as "%Hreg";eauto.
-  rewrite !big_sepM_insert ?big_sepM_empty;eauto.
-  iFrame.
-  apply lookup_insert_None; split;eauto; intros P; by inversion P.
-  iPureIntro.
-  split.
-  - by apply (Hreg (r1, i) w1 (lookup_insert _ (r1, i) w1)).
-  - apply (Hreg (r2, i) w2);eauto.
-    rewrite lookup_insert_Some;right;split;
-    [intros P; inversion P; contradiction|];
-    by rewrite !lookup_insert.
- Qed.
-
+  Lemma gen_reg_valid2:
+   ∀ (σ : state) i r1 w1 r2 w2 ,
+     (get_current_vm σ) = i ->
+     r1 ≠ r2->
+     ghost_map_auth (gen_reg_name vmG) 1 (get_reg_gmap σ) -∗
+     r1 @@ i ->r w1 -∗
+     r2 @@ i ->r w2 -∗
+     ⌜ (get_reg σ r1) = Some w1 ⌝ ∗ ⌜ (get_reg σ r2) =Some w2 ⌝.
+  Proof.
+    iIntros (?????? Hneq Hi) "Hreg Hr1 Hr2".
+    iDestruct ((gen_reg_valid_Sep σ i (<[(r1,i):=w1]>{[(r2,i):=w2]}))
+                 with "Hreg [Hr1 Hr2]") as "%Hreg";eauto.
+    rewrite !big_sepM_insert ?big_sepM_empty;eauto.
+    iFrame.
+    apply lookup_insert_None; split;eauto; intros P; by inversion P.
+    iPureIntro.
+    split.
+    - by apply (Hreg (r1, i) w1 (lookup_insert _ (r1, i) w1)).
+    - apply (Hreg (r2, i) w2);eauto.
+      rewrite lookup_insert_Some;right;split;
+      [intros P; inversion P; contradiction|];
+      by rewrite !lookup_insert.
+  Qed.
 
 Lemma gen_reg_valid3:
   ∀ (σ : state) i r1 w1 r2 w2 r3 w3 ,
@@ -565,7 +576,7 @@ Lemma gen_reg_valid3:
     r1 @@ i ->r w1 -∗
     r2 @@ i ->r w2 -∗
     r3 @@ i ->r w3 -∗
-                ⌜ (get_reg σ r1) = Some w1 ⌝ ∗ ⌜ (get_reg σ r2) =Some w2 ⌝ ∗ ⌜ (get_reg σ r3) = Some w3⌝.
+    ⌜ (get_reg σ r1) = Some w1 ⌝ ∗ ⌜ (get_reg σ r2) =Some w2 ⌝ ∗ ⌜ (get_reg σ r3) = Some w3⌝.
 Proof.
   iIntros (???????? Hi Hneq1 Hneq2 Hneq3) "Hreg Hr1 Hr2 Hr3".
   iDestruct ((gen_reg_valid_Sep σ i ({[(r1,i):=w1;(r2,i):=w2;(r3,i):=w3]}))
@@ -643,8 +654,6 @@ Proof.
     by rewrite !lookup_insert.
 Qed.
 
-
-
 Lemma gen_reg_update1_global:
   ∀ (σ : state) r i w w',
     ghost_map_auth (gen_reg_name vmG) 1 (get_reg_gmap σ) -∗
@@ -659,25 +668,23 @@ Lemma gen_reg_update1_global:
   done.
  Qed.
 
-
  Lemma reg_proper {m: gmap (reg_name * VMID) Word}:
-([∗ map] k ↦ x ∈ m, k↪[gen_reg_name vmG] x) ⊣⊢ ([∗ map]k ↦ x ∈ m,  (k.1, k.2)↪[gen_reg_name vmG] x).
-   Proof.
-      iApply (big_sepM_proper _ (λ k x, (k.1, k.2)↪[gen_reg_name vmG] x)%I).
-      intros.
-  simpl.
-  f_equiv.
-  destruct k;done.
-Qed.
-
+ ([∗ map] k ↦ x ∈ m, k↪[gen_reg_name vmG] x) ⊣⊢ ([∗ map]k ↦ x ∈ m,  (k.1, k.2)↪[gen_reg_name vmG] x).
+ Proof.
+   iApply (big_sepM_proper _ (λ k x, (k.1, k.2)↪[gen_reg_name vmG] x)%I).
+   intros.
+   simpl.
+   f_equiv.
+   destruct k;done.
+ Qed.
 
  Lemma gen_reg_update_Sep:
   ∀ (σ : state) regs regs',
-      dom (gset (reg_name * VMID)) regs = dom (gset (reg_name * VMID )) regs' ->
+    dom (gset (reg_name * VMID)) regs = dom (gset (reg_name * VMID )) regs' ->
     ghost_map_auth (gen_reg_name vmG) 1 (get_reg_gmap σ) -∗
     ([∗ map] r↦w ∈ regs,  r.1 @@ r.2 ->r w) ==∗
-               ghost_map_auth (gen_reg_name vmG) 1 (regs' ∪ (get_reg_gmap σ)) ∗
-             ([∗ map] r↦w ∈ regs',  r.1 @@ r.2 ->r w).
+    ghost_map_auth (gen_reg_name vmG) 1 (regs' ∪ (get_reg_gmap σ)) ∗
+    ([∗ map] r↦w ∈ regs',  r.1 @@ r.2 ->r w).
  Proof.
   iIntros (????) "Hσ Hr".
   rewrite reg_mapsto_eq /reg_mapsto_def.
@@ -693,27 +700,27 @@ Qed.
   ∀ (σ : state) r1 i1 w1 w1' r2 i2 w2 w2',
     r1 ≠ r2 ∨ i1 ≠ i2 ->
     ghost_map_auth (gen_reg_name vmG) 1 (get_reg_gmap σ) -∗
-     r1 @@ i1 ->r w1 -∗
-                      r2 @@ i2 ->r w2==∗
-               ghost_map_auth (gen_reg_name vmG) 1 (<[(r1,i1) := w1']> (<[(r2,i2) := w2']> (get_reg_gmap σ))) ∗
-             r1 @@ i1 ->r w1'  ∗ r2 @@ i2 ->r w2'.
+    r1 @@ i1 ->r w1 -∗
+    r2 @@ i2 ->r w2==∗
+    ghost_map_auth (gen_reg_name vmG) 1 (<[(r1,i1) := w1']> (<[(r2,i2) := w2']> (get_reg_gmap σ))) ∗
+    r1 @@ i1 ->r w1' ∗ r2 @@ i2 ->r w2'.
  Proof.
   iIntros (????????? Hneq) "Hreg Hr1 Hr2".
   iDestruct ((gen_reg_update_Sep _ {[(r1,i1):=w1; (r2,i2):=w2]} {[(r1,i1):=w1'; (r2,i2):=w2']}) with "Hreg [Hr1 Hr2]")
     as ">[Hreg Hr12]" ;eauto;[set_solver| | ].
-        rewrite !big_sepM_insert ?big_sepM_empty;eauto.
-        iFrame.
-        destruct Hneq; apply lookup_insert_None; split;eauto; intros P; by inversion P.
-        iModIntro.
-        rewrite !big_sepM_insert ?big_sepM_empty;eauto.
-        iDestruct "Hr12" as "(? & ? & _)".
-        rewrite ?insert_union_singleton_l map_union_assoc.
-        simplify_map_eq.
-        by iFrame.
-        destruct Hneq; apply lookup_insert_None; split;eauto; intros P; by inversion P.
-Qed.
+  rewrite !big_sepM_insert ?big_sepM_empty;eauto.
+  iFrame.
+  destruct Hneq; apply lookup_insert_None; split;eauto; intros P; by inversion P.
+  iModIntro.
+  rewrite !big_sepM_insert ?big_sepM_empty;eauto.
+  iDestruct "Hr12" as "(? & ? & _)".
+  rewrite ?insert_union_singleton_l map_union_assoc.
+  simplify_map_eq.
+  by iFrame.
+  destruct Hneq; apply lookup_insert_None; split;eauto; intros P; by inversion P.
+ Qed.
 
-  Lemma gen_reg_update3_global {σ w1 w2 w3} r1 i1 w1' r2 i2 w2' r3 i3 w3':
+ Lemma gen_reg_update3_global {σ w1 w2 w3} r1 i1 w1' r2 i2 w2' r3 i3 w3':
     r1 ≠ r2 ∨ i1 ≠ i2  ->
     r1 ≠ r3 ∨ i1 ≠ i3  ->
     r3 ≠ r2 ∨ i3 ≠ i2  ->
@@ -727,51 +734,56 @@ Qed.
   iIntros (Hneq12 Hneq13 Hneq32) "Hreg Hr1 Hr2 Hr3".
   iDestruct ((gen_reg_update_Sep _ {[(r1,i1):=w1; (r2,i2):=w2 ;(r3,i3):=w3]} {[(r1,i1):=w1'; (r2,i2):=w2'; (r3,i3):=w3']}) with "Hreg [Hr1 Hr2 Hr3]")
     as ">[Hreg Hr123]" ;eauto;[set_solver| | ].
-        rewrite !big_sepM_insert ?big_sepM_empty;eauto.
-        iFrame.
-        destruct Hneq32; apply lookup_insert_None; split;eauto; intros P; by inversion P.
-        destruct Hneq12; apply lookup_insert_None; split;eauto.
-        destruct Hneq13; apply lookup_insert_None; split;eauto; intros P; by inversion P.
-        intros P; by inversion P.
-        destruct Hneq13; apply lookup_insert_None; split;eauto; intros P; by inversion P.
-        intros P; by inversion P.
-        iModIntro.
-        rewrite !big_sepM_insert ?big_sepM_empty;eauto.
-        iDestruct "Hr123" as "(? & ? & ? & _)".
-        rewrite ?insert_union_singleton_l !map_union_assoc.
-        simplify_map_eq.
-        by iFrame.
-        destruct Hneq32; apply lookup_insert_None; split;eauto; intros P; by inversion P.
-        destruct Hneq12; apply lookup_insert_None; split;eauto.
-        destruct Hneq13; apply lookup_insert_None; split;eauto; intros P; by inversion P.
-        intros P; by inversion P.
-        destruct Hneq13; apply lookup_insert_None; split;eauto; intros P; by inversion P.
-        intros P; by inversion P.
-Qed.
-
-
+  rewrite !big_sepM_insert ?big_sepM_empty;eauto.
+  iFrame.
+  destruct Hneq32; apply lookup_insert_None; split;eauto; intros P; by inversion P.
+  destruct Hneq12; apply lookup_insert_None; split;eauto.
+  destruct Hneq13; apply lookup_insert_None; split;eauto; intros P; by inversion P.
+  intros P; by inversion P.
+  destruct Hneq13; apply lookup_insert_None; split;eauto; intros P; by inversion P.
+  intros P; by inversion P.
+  iModIntro.
+  rewrite !big_sepM_insert ?big_sepM_empty;eauto.
+  iDestruct "Hr123" as "(? & ? & ? & _)".
+  rewrite ?insert_union_singleton_l !map_union_assoc.
+  simplify_map_eq.
+  by iFrame.
+  destruct Hneq32; apply lookup_insert_None; split;eauto; intros P; by inversion P.
+  destruct Hneq12; apply lookup_insert_None; split;eauto.
+  destruct Hneq13; apply lookup_insert_None; split;eauto; intros P; by inversion P.
+  intros P; by inversion P.
+  destruct Hneq13; apply lookup_insert_None; split;eauto; intros P; by inversion P.
+  intros P; by inversion P.
+ Qed.
 
  (* rules for memory points-to *)
-  Lemma mem_dupl_false a w1 w2:
+ Lemma mem_dupl_false a w1 w2:
    a ->a w1 -∗ a ->a w2 -∗ False.
-  Proof using.
+ Proof using.
     rewrite mem_mapsto_eq /mem_mapsto_def.
     iIntros "Ha1 Ha2".
     iDestruct (ghost_map_elem_valid_2 with "Ha1 Ha2") as %?.
     destruct H.
     apply dfrac_valid_own_r in H.
     inversion H.
-  Qed.
+ Qed.
 
-  Lemma mem_neq a1 a2  w1 w2:
+ Lemma mem_neq a1 a2  w1 w2:
    a1 ->a w1 -∗ a2 ->a w2 -∗ ⌜ a1 <> a2⌝.
-  Proof using.
+ Proof using.
     iIntros "Ha1 Ha2".
     destruct (decide (a1 = a2)).
     - simplify_eq /=.
       iDestruct (mem_dupl_false with "Ha1 Ha2") as %[].
     - done.
-  Qed.
+ Qed.
+
+ Lemma gen_mem_alloc (mem: gmap Addr Word) :
+   ⊢ |==> ∃ γ, ghost_map_auth γ 1 mem ∗
+               [∗ map] p↦w∈ mem, ghost_map_elem γ p (DfracOwn 1) w.
+ Proof.
+   iApply (ghost_map_alloc mem).
+ Qed.
 
 Lemma gen_mem_valid:
   ∀ (σ : state) a w,
@@ -850,7 +862,6 @@ Proof.
     by simplify_map_eq.
  Qed.
 
-
 Lemma gen_mem_update1:
   ∀ (σ : state) a w w',
     ghost_map_auth (gen_mem_name vmG) 1 (get_mem σ) -∗
@@ -880,46 +891,6 @@ Definition mem_page (instr: list Word) (p: PID):=
 (*      | None => ∃ w, (a->a w) *)
 (*    end)%I. *)
 
-
-Lemma finz_seq_lookup0{b} n (f : finz.finz b) x :
-   is_Some(f + 1)%f ->
-   finz.seq f n !! x = Some f -> x=0.
-Proof.
-  revert f. destruct n; cbn.
-  { intros. inversion H0. }
-  { intros.
-    destruct (decide (x=0)).
-    done.
-    rewrite lookup_cons_ne_0 in H0.
-    apply elem_of_list_lookup_2 in H0.
-    pose proof (finz_seq_notin _ f (f ^+ 1)%f n).
-    assert ( (f < f ^+ 1)%f) as Hlt.
-    solve_finz.
-    apply H1 in Hlt.
-    done.
-    done. }
-Qed.
-
-
-Lemma finz_seq_NoDup'{b} (f : finz.finz b) (n : nat) :
-  is_Some (f + (Z.of_nat (n-1)))%f →
-  NoDup (finz.seq f n).
-Proof using.
-  revert f. induction n; intros f Hfn.
-  { apply NoDup_nil_2. }
-  { cbn.
-    destruct n; intros;simpl.
-    { apply NoDup_singleton. }
-    { apply NoDup_cons_2.
-      apply not_elem_of_cons.
-      split.
-      solve_finz.
-      apply finz_seq_notin.
-      solve_finz.
-      eapply IHn.
-      solve_finz. } }
-Qed.
-
 Lemma gen_mem_update_Sep_list{ σ} (ads : list Addr) (ws ws': list Word):
  NoDup ads ->
  length ws = length ws' ->
@@ -943,7 +914,6 @@ Proof.
   iFrame.
   iModIntro. iPureIntro. lia.
 Qed.
-
 
 Lemma gen_mem_update_page{σ ws} p (ws': list Word):
  length ws' = (Z.to_nat page_size) ->
@@ -1062,7 +1032,6 @@ Proof.
   }
 Qed.
 
-
 Lemma list2_pid_words_in p ps wss:
   p ∈ ps ->
    ([∗ list] p;ws ∈ ps;wss, mem_page ws p) ⊢
@@ -1131,7 +1100,6 @@ Proof.
     done.
     }
 Qed.
-
 
 Lemma mem_page_list_list (ps: list PID) (wss: list (list Word)):
  ([∗ list] p;ws ∈ ps;wss, mem_page ws p) -∗
@@ -1215,8 +1183,32 @@ Qed.
    done.
  Qed.
 
+ Lemma gen_tx_alloc (gm : (gmap VMID (agreeR (leibnizO PID)))) :
+  ✓ gm ->
+  ⊢ |==> ∃ γ, own γ (● gm) ∗ own γ (◯ gm).
+ Proof.
+   iIntros.
+   iDestruct (own_alloc ((● gm) ⋅ (◯ gm ))) as ">Halloc".
+   { apply auth_both_valid_discrete. split;done. }
+   iModIntro.
+   iDestruct "Halloc" as (γ) "Halloc".
+   iExists γ.
+   rewrite own_op //.
+ Qed.
+
+ Lemma get_txrx_auth_agree_valid σ f:
+  ✓ (get_txrx_auth_agree σ f).
+ Proof.
+   rewrite /get_txrx_auth_agree.
+   induction list_of_vmids;cbn.
+   done.
+   apply (insert_valid _ a ((to_agree (f (get_vm_mail_box σ a))): (agreeR (leibnizO PID)))).
+   { done. }
+   apply IHl.
+ Qed.
+
  Lemma gen_tx_valid σ i p:
-  TX@ i := p -∗ own (gen_tx_name vmG) (get_tx_agree σ) -∗ ⌜ (get_vm_mail_box σ i).1 = p ⌝.
+  TX@ i := p -∗ own (gen_tx_name vmG) (● (get_tx_agree σ)) -∗ ⌜ (get_vm_mail_box σ i).1 = p ⌝.
  Proof.
    iIntros "Htx Hσ".
    rewrite tx_mapsto_eq /tx_mapsto_def.
@@ -1273,155 +1265,131 @@ Qed.
 
 
   (* rules for RX *)
-  Lemma rx_split_some i p n (v: VMID):
+ Lemma rx_split_some i p n (v: VMID):
   RX@ i :=( p ! n , v)  -∗ RX@ i :=( p ! n, v)  ∗ RX@ i := p.
-  Proof using.
-    iIntros "HR".
-    rewrite rx_mapsto_eq1 rx_mapsto_eq2.
-    iApply own_op.
-    rewrite -pair_op -auth_frag_op.
-    rewrite singleton_op agree_idemp.
-    rewrite Some_op_opM.
-    simplify_eq /=.
-    done.
-  Qed.
+ Proof using.
+   iIntros "[HRa HRo]".
+   rewrite rx_agree_mapsto_eq rx_option_mapsto_eq.
+   iFrame "HRo".
+   iApply own_op.
+   rewrite -auth_frag_op.
+   rewrite singleton_op agree_idemp.
+   simplify_eq /=.
+   done.
+ Qed.
 
-  Lemma rx_split_none i p:
+ Lemma rx_split_none i p:
   RX@ i :=(p !) -∗ RX@ i :=(p !) ∗ RX@ i := p.
-  Proof using.
-    iIntros "HR".
-    rewrite rx_mapsto_eq1 rx_mapsto_eq2.
-    iApply own_op.
-    rewrite -pair_op -auth_frag_op.
-    rewrite singleton_op agree_idemp.
-    rewrite  Some_op_opM.
-    simplify_eq /=.
-    done.
-  Qed.
+ Proof using.
+   iIntros "[HRa HRo]".
+   rewrite rx_agree_mapsto_eq rx_option_mapsto_eq.
+   iFrame "HRo".
+   iApply own_op.
+   rewrite -auth_frag_op.
+   rewrite singleton_op agree_idemp.
+   simplify_eq /=.
+   done.
+ Qed.
 
-  Lemma rx_dupl i p:
+ Lemma rx_dupl i p:
    RX@i:=p -∗ RX@i:=p ∗ RX@i:=p.
-  Proof using.
-    iIntros "HR".
-    rewrite rx_mapsto_eq2.
-    iApply own_op.
-    rewrite -pair_op -auth_frag_op.
-    rewrite singleton_op agree_idemp.
-    naive_solver.
+ Proof using.
+   iIntros "HR".
+   rewrite rx_agree_mapsto_eq.
+   iApply own_op.
+   rewrite -auth_frag_op.
+   rewrite singleton_op agree_idemp.
+   naive_solver.
+ Qed.
+  
+ Definition gen_rx_agree_alloc := gen_tx_alloc.
+ 
+ Lemma gen_rx_option_alloc (gmo: gmap VMID (option (Word * VMID))):
+  ⊢ |==> ∃ γ, ghost_map_auth γ 1 gmo ∗
+                             [∗ map] k ↦ v∈ gmo, ghost_map_elem γ k (DfracOwn 1) v.
+ Proof.
+   iIntros.
+   iApply (ghost_map_alloc gmo).
+ Qed.
+
+ Lemma gen_rx_agree_valid σ i p:
+  ✓ (● get_rx_agree σ ⋅ ◯ {[i := to_agree p]}) -> (get_vm_mail_box σ i).2.1 = p.
+ Proof.
+   intro.
+   rewrite /get_rx_agree /get_txrx_auth_agree in H.
+   apply auth_both_valid_discrete in H;destruct H as [H _].
+   remember  ((list_to_map (map (λ v : VMID, (v, to_agree (get_vm_mail_box σ v).2.1)) list_of_vmids)): gmap VMID (agreeR (leibnizO PID))) as m.
+   rewrite -> (lookup_included {[i := to_agree p]} m) in H.
+   pose proof (H i).
+   clear H.
+   simplify_map_eq /=.
+   apply option_included_total in H0;destruct H0.
+   rewrite -> (lookup_singleton_None i i (to_agree p)) in H;done.
+   destruct H as [x [x0 [H H0]]].
+   rewrite -> (lookup_singleton_Some i i (to_agree p)) in H.
+   inversion H; subst x;clear H H1.
+   destruct H0.
+   apply elem_of_list_to_map_2 in H.
+   apply elem_of_list_In in H.
+   apply in_map_iff in H.
+   inversion H;clear H.
+   destruct H1 as [H1 _];inversion H1;subst;clear H1.
+   rewrite -> (to_agree_included (p: (leibnizO PID)) _) in H0.
+   by fold_leibniz.
+ Qed.
+
+
+ Lemma gen_rx_pid_valid σ i p:
+  RX@ i := p -∗ own (gen_rx_agree_name vmG) (● (get_rx_agree σ))-∗ ⌜ (get_vm_mail_box σ i).2.1 = p ⌝.
+ Proof.
+   iIntros "Hrx Hσ".
+   rewrite rx_agree_mapsto_eq /rx_agree_mapsto_def.
+   iDestruct (own_valid_2 with "Hσ Hrx") as %?.
+   iPureIntro.
+   by apply gen_rx_agree_valid.
+ Qed.
+
+ Lemma gen_rx_none_valid σ i p:
+  RX@ i :=( p !) -∗
+  ghost_map_auth (gen_rx_option_name vmG) 1 (get_rx_gmap σ)-∗
+  ⌜ (get_vm_mail_box σ i).2.2 = None⌝.
+ Proof.
+   iIntros "[_ Hrx] Hσ".
+   rewrite rx_option_mapsto_eq /rx_option_mapsto_def.
+   iDestruct (ghost_map_lookup with "Hσ Hrx") as "%".
+   rewrite /get_rx_gmap in H.
+   apply elem_of_list_to_map_2 in H.
+   apply elem_of_list_In in H.
+   apply in_map_iff in H.
+   destruct H as [x [H _]].
+   destruct ((get_vm_mail_box σ x).2.2) eqn:Heqn.
+   destruct p0;inversion H.
+   inversion H;subst.
+   iPureIntro.
+   rewrite -Heqn //.
+ Qed.
+
+ Lemma gen_rx_valid_some σ i p l v:
+  RX@ i :=( p ! l , v) -∗
+  ghost_map_auth (gen_rx_option_name vmG) 1 (get_rx_gmap σ)-∗
+  ⌜ (get_vm_mail_box σ  i).2.2 = Some(l,v)⌝.
+ Proof.
+    iIntros "[_ Hrx] Hσ".
+    rewrite rx_option_mapsto_eq /rx_option_mapsto_def.
+    iDestruct (ghost_map_lookup with "Hσ Hrx") as "%".
+   rewrite /get_rx_gmap in H.
+   apply elem_of_list_to_map_2 in H.
+   apply elem_of_list_In in H.
+   apply in_map_iff in H.
+   destruct H as [x [H _]].
+   destruct ((get_vm_mail_box σ x).2.2) eqn:Heqn.
+   destruct p0;inversion H.
+   inversion H;subst.
+   iPureIntro.
+   rewrite -Heqn //.
+   inversion H.
   Qed.
 
-
-  Lemma gen_rx_agree_valid σ i p:
-   ✓ (get_rx_agree σ ⋅ ◯ {[i := to_agree p]}) -> (get_vm_mail_box σ i).2.1 = p.
-  Proof.
-    intro.
-    rewrite /get_rx_agree /get_txrx_auth_agree in H.
-    apply auth_both_valid_discrete in H;destruct H as [H _].
-    remember  ((list_to_map (map (λ v : VMID, (v, to_agree (get_vm_mail_box σ v).2.1)) list_of_vmids)): gmap VMID (agreeR (leibnizO PID))) as m.
-    rewrite -Heqm in H.
-    rewrite -> (lookup_included {[i := to_agree p]} m) in H.
-    pose proof (H i).
-    clear H.
-    simplify_map_eq /=.
-    apply option_included_total in H0;destruct H0.
-    rewrite -> (lookup_singleton_None i i (to_agree p)) in H;done.
-    destruct H as [x [x0 [H H0]]].
-    rewrite -> (lookup_singleton_Some i i (to_agree p)) in H.
-    inversion H; subst x;clear H H1.
-    destruct H0.
-    apply elem_of_list_to_map_2 in H.
-    apply elem_of_list_In in H.
-    apply in_map_iff in H.
-    inversion H;clear H.
-    destruct H1 as [H1 _];inversion H1;subst;clear H1.
-    rewrite -> (to_agree_included (p: (leibnizO PID)) _) in H0.
-    by fold_leibniz.
-  Qed.
-
-
-  Lemma gen_rx_pid_valid σ i p:
-   RX@ i := p -∗ own (gen_rx_name vmG) ((get_rx_agree σ), (get_rx_gmap σ) )-∗ ⌜ (get_vm_mail_box σ i).2.1 = p ⌝.
-  Proof.
-    iIntros "Hrx Hσ".
-    rewrite rx_mapsto_eq2 /rx_mapsto_def2 .
-    iDestruct (own_valid_2  with "Hσ Hrx") as %?.
-    iPureIntro.
-    rewrite -pair_op in H.
-    apply pair_valid in H; destruct H as [H _].
-    simpl in H.
-    by apply gen_rx_agree_valid.
-  Qed.
-
-  Lemma gen_rx_gmap_none_valid σ i:
-  ✓ (get_rx_gmap σ ⋅ Some (gmap_view_frag i (DfracOwn 1) None)) -> (get_vm_mail_box σ i).2.2 = None.
-  Proof.
-    intro.
-    rewrite /get_rx_gmap -Some_op in H.
-    rewrite -> Some_valid in H.
-    apply gmap_view_both_frac_valid_L in H as [_ [_ H]].
-    apply elem_of_list_to_map_2 in H.
-    apply elem_of_list_In in H.
-    apply in_map_iff in H.
-    destruct H as [x [H _]].
-    destruct ((get_vm_mail_box σ x).2.2) eqn:Heqn.
-    destruct p;inversion H.
-    inversion H;subst.
-    by inversion H.
-  Qed.
-
-  Lemma gen_rx_none_valid σ i p:
-   RX@ i :=( p !) -∗
-   own (gen_rx_name vmG) ((get_rx_agree σ), (get_rx_gmap σ) )-∗
-   ⌜ (get_vm_mail_box σ i).2 = (p,None)  ⌝.
-  Proof.
-    iIntros "Hrx Hσ".
-    rewrite rx_mapsto_eq1 /rx_mapsto_def1.
-    iDestruct (own_valid_2 with "Hσ Hrx") as %?.
-    iPureIntro.
-    rewrite -pair_op in H.
-    apply pair_valid in H; destruct H as [Hagree Hgmap];simpl in Hagree;simpl in Hgmap.
-    apply gen_rx_agree_valid in Hagree.
-    apply gen_rx_gmap_none_valid in Hgmap.
-    destruct ((get_vm_mail_box σ i).2) eqn:Heqn.
-    rewrite -Hagree -Hgmap.
-    done.
-  Qed.
-
-
-  Lemma gen_rx_gmap_some_valid σ i l v:
-  ✓ (get_rx_gmap σ ⋅ Some (gmap_view_frag i (DfracOwn 1) (Some(l,v)))) -> (get_vm_mail_box σ i).2.2 = Some(l,v).
-  Proof.
-    intro.
-    rewrite /get_rx_gmap -Some_op in H.
-    rewrite -> Some_valid in H.
-    apply gmap_view_both_frac_valid_L in H as [_ [_ H]].
-    apply elem_of_list_to_map_2 in H.
-    apply elem_of_list_In in H.
-    apply in_map_iff in H.
-    destruct H as [x [H _]].
-    destruct ((get_vm_mail_box σ x).2.2) eqn:Heqn.
-    by destruct p;inversion H;subst.
-    by inversion H.
-  Qed.
-
-
-  Lemma gen_rx_valid_some σ i p l v:
-   RX@ i :=( p ! l , v) -∗
-   own (gen_rx_name vmG) ((get_rx_agree σ), (get_rx_gmap σ) )-∗
-   ⌜ (get_vm_mail_box σ i).2 = (p,Some(l,v))⌝.
-  Proof.
-    iIntros "Hrx Hσ".
-    rewrite rx_mapsto_eq1 /rx_mapsto_def1.
-    iDestruct (own_valid_2 with "Hσ Hrx") as %?.
-    iPureIntro.
-    rewrite -pair_op in H.
-    apply pair_valid in H; destruct H as [Hagree Hgmap];simpl in Hagree;simpl in Hgmap.
-    apply gen_rx_agree_valid in Hagree.
-    apply gen_rx_gmap_some_valid in Hgmap.
-    destruct ((get_vm_mail_box σ i).2) eqn:Heqn.
-    rewrite -Hagree -Hgmap.
-    done.
-  Qed.
 (*
   (* rules for pagetables  *)
   Lemma owned_split_set i q1 q2 (s1 s2 : gset PID):
@@ -1466,6 +1434,8 @@ Qed.
     done.
   Qed.
 *)
+
+ (* TODO: alloc lemmas *)
 
 Lemma gen_pagetable_valid_lookup_Set{Perm: Type} {σ i q γ} proj (checkb: Perm -> bool) (s:gset PID):
     own γ (● (get_pagetable_gmap σ proj checkb))  -∗
@@ -2016,14 +1986,14 @@ Proof. rewrite excl_mapsto_eq /excl_mapsto_def. apply _. Qed.
 Global Instance tx_mapsto_timeless i p : Timeless (TX@ i := p).
 Proof. rewrite tx_mapsto_eq /tx_mapsto_def. apply _. Qed.
 
-Global Instance rx_mapsto_timeless1 i p n (r:VMID) : Timeless (RX@ i :=(p ! n , r )).
-Proof. rewrite rx_mapsto_eq1 /rx_mapsto_def1. apply _. Qed.
+Global Instance rx_mapsto_timeless1 i p : Timeless (RX@ i :=p).
+Proof. rewrite rx_agree_mapsto_eq /rx_agree_mapsto_def. apply _. Qed.
 
-Global Instance rx_mapsto_timeless2 i p : Timeless (RX@ i :=(p !)).
-Proof. rewrite rx_mapsto_eq1 /rx_mapsto_def1. apply _. Qed.
+Global Instance rx_mapsto_timeless2 i p n (r:VMID) : Timeless (RX@ i :=(p ! n , r )).
+Proof. rewrite rx_option_mapsto_eq /rx_option_mapsto_def. apply _. Qed.
 
-Global Instance rx_mapsto_timeless3 i p : Timeless (RX@ i :=p).
-Proof. rewrite rx_mapsto_eq2 /rx_mapsto_def2. apply _. Qed.
+Global Instance rx_mapsto_timeless3 i p : Timeless (RX@ i :=(p !)).
+Proof. rewrite rx_option_mapsto_eq /rx_option_mapsto_def. apply _. Qed.
 
 Global Instance trans_mapsto_timeless w q v x y m f : Timeless (w ->t{ q }( v , x , y , m , f )).
 Proof. rewrite trans_mapsto_eq /trans_mapsto_def. apply _. Qed.
