theories/rules/br.v
@@ -22,7 +22,7 @@ Proof.
   inversion Hsche as [ Hcur ]; clear Hsche.
   apply fin_to_nat_inj in Hcur.
   iModIntro.
-  iDestruct "Hσ" as "(? & Hmem & Hreg & ? & ? & ? & Haccess & ?)".
+  iDestruct "Hσ" as "(? & Hmem & Hreg & ? & ? & ? & ? & Haccess & ?)".
   pose proof (decode_instruction_valid w1 instr Hdecode) as Hvalidinstr.
   rewrite Hinstr in Hvalidinstr.
   inversion Hvalidinstr as [ | | | | | | |src Hvalidra] .
