theories/rules/fail.v
@@ -22,7 +22,7 @@ Proof.
   inversion Hsche as [ Hcur ]; clear Hsche.
   apply fin_to_nat_inj in Hcur.
   iModIntro.
-  iDestruct "Hσ" as "(? & Hmem & Hreg & ? & ? & ? & Haccess & ?)".
+  iDestruct "Hσ" as "(? & Hmem & Hreg & ? & ? & ? & ? & Haccess & ?)".
   (* valid regs *)
   iDestruct ((gen_reg_valid1 σ1 PC i ai Hcur ) with "Hreg Hpc") as "%HPC";eauto.
   (* valid pt *)
